LeroyCompilerVerificationCourse/Sequences.lean
@@ -26,50 +26,40 @@ info: infseq.coinduct.{u_1} {α : Sort u_1} (R : α → α → Prop) (x : α →
 #guard_msgs in #check infseq.coinduct
 
 -- Simple proof by coinduction
-theorem cycle_infseq {R : α → α → Prop} (x : α) : R x x → infseq R x := by
-  apply infseq.coinduct R (λ m => R m m)
-  grind
+theorem cycle_infseq {R : α → α → Prop} (x : α) : R x x → infseq R x :=
+  infseq.coinduct R (λ m => R m m) (by grind) _
 
 @[grind] inductive star (R : α → α → Prop) : α → α → Prop where
   | star_refl : ∀ x : α, star R x x
-  | star_step : ∀ x y z, R x y → star R y z → star R x z
+  | star_step : ∀ {x y z}, R x y → star R y z → star R x z
 
-@[grind] theorem star_one (R : α → α → Prop) : ∀ a b : α, R a b → star R a b := by
-  intros a b Rab
-  apply star.star_step
-  exact Rab
-  grind
+-- Whenever we have `star R y z` and want to prove `star R x z`, look for `R x y`:
+attribute [grind =>] star.star_step
 
-@[grind] theorem star_trans {α} (R : α → α → Prop) : ∀ (a b : α), star R a b → ∀ c : α, star R b c → star R a c := by
-  intros a b sab
-  intro c
-  intro sbc
-  induction sab
-  case star_refl => exact sbc
-  case star_step rel m ih =>
-    apply star.star_step
-    exact rel
-    grind
+@[grind] theorem star_one (R : α → α → Prop) {a b : α} (h : R a b) : star R a b :=
+  star.star_step h (by grind)
 
+@[grind] theorem star_trans {α} (R : α → α → Prop) (a b : α) (sab : star R a b) : ∀ c : α, star R b c → star R a c := by
+  induction sab with grind
+
+@[grind cases]
 inductive plus (R : α → α → Prop) : α → α → Prop where
-| plus_left : ∀ a b c, R a b → star R b c → plus R a c
+| plus_left : ∀ {a b c}, R a b → star R b c → plus R a c
 
-theorem plus_one : ∀ a b, R a b → plus R a b := by
-  intro a b Rab
-  apply plus.plus_left
-  · exact Rab
-  · grind
+-- Whenever we have `star R b c` and want to prove `plus R a c`, look for `R a b`:
+grind_pattern plus.plus_left => star R b c, plus R a c
 
-@[grind] theorem plus_star : ∀ a b, plus R a b → star R a b := by
-    intro a b h
-    cases h
-    case plus_left h₁ h₂ h₃ =>
-      grind [star.star_step]
+@[grind ←]
+theorem plus_one {a b} (h : R a b) : plus R a b :=
+  plus.plus_left h (by grind)
+
+@[grind] theorem plus_star {a b} (h : plus R a b) : star R a b := by
+    grind
 
 @[grind] theorem plus_star_trans (R : α → α → Prop) : ∀ (a b c : α), star R a b → plus R b c → plus R a c := by
   intro a b c s p
   induction s
-  any_goals grind
+  case star_refl => grind
   case star_step d e f rel s2 ih =>
     apply plus.plus_left
     exact rel
@@ -86,11 +76,9 @@ theorem star_plus_trans :
       · exact a1
       · grind
 
-theorem plus_right :
-  ∀ a b c, star R a b -> R b c -> plus R a c := by
-  intro a b c h₁ h₂
-  grind [star_plus_trans, plus_one]
+-- grind_pattern star_plus_trans => star R a b, plus R b c
 
+theorem plus_right : star R a b -> R b c -> plus R a c := by grind
 
 def all_seq_inf (R : α → α → Prop) (x : α) : Prop :=
   ∀ y : α, star R x y → ∃ z, R y z
@@ -101,7 +89,7 @@ def infseq_with_function (R : α → α → Prop) (a: α) : Prop :=
 def infseq_if_all_seq_inf (R : α → α → Prop) : ∀ x, all_seq_inf R x → infseq R x := by
   apply infseq.coinduct
   intro x H
-  apply Exists.elim (H x (by simp only [star.star_refl]))
+  apply Exists.elim (H x (by grind))
   intro y Rxy
   exists y
   constructor
@@ -111,15 +99,9 @@ def infseq_if_all_seq_inf (R : α → α → Prop) : ∀ x, all_seq_inf R x → 
     apply H
     grind
 
-theorem infseq_coinduction_principle_2 :
-  ∀ (x : α → Prop),
-  (∀ (a : α), x a → ∃ b, plus R a b ∧ x b) →
-  ∀ (a : α), x a → infseq R a := by
-    intro X
-    intro h₁ a rel
-    apply infseq.coinduct _ (fun a => ∃ b, star R a b ∧ X b)
-    case x => grind
-    case y => grind [cases plus]
+theorem infseq_coinduction_principle_2
+    (X : α → Prop) (h₁ : ∀ (a : α), X a → ∃ b, plus R a b ∧ X b) (a : α) (rel : X a) : infseq R a := by
+  apply infseq.coinduct _ (fun a => ∃ b, star R a b ∧ X b) <;> grind
 
 theorem infseq_from_function : ∀ a, infseq_with_function R a → infseq R a := by
   apply infseq.coinduct
@@ -129,41 +111,31 @@ theorem infseq_from_function : ∀ a, infseq_with_function R a → infseq R a :=
   refine ⟨f 1, ?_⟩
   refine ⟨by grind, ?_⟩
   unfold infseq_with_function
-  refine ⟨fun n => f (n + 1), ?_⟩
-  refine ⟨by grind, ?_⟩
-  intro i
-  specialize hsucc (i + 1)
-  grind
+  refine ⟨fun n => f (n + 1), by grind⟩
 
 @[grind] def irred (R : α → α → Prop) (a : α) : Prop := ∀ b, ¬(R a b)
 
-theorem star_star_inv (R_functional : ∀ a b c, R a b -> R a c -> b = c) : ∀ a b, star R a b -> forall c, star R a c → star R b c ∨ star R c b := by
-  intro _ _ sab
+theorem star_star_inv (R_functional : ∀ a b c, R a b -> R a c -> b = c) (sab : star R a b) :
+    ∀ c, star R a c → star R b c ∨ star R c b := by
   induction sab <;> grind
 
 theorem finseq_unique (R_functional : ∀ a b c, R a b -> R a c -> b = c) :
   ∀ a b b', star R a b → irred R b → star R a b' → irred R b' → b = b' := by
     intro a b b' sab ib sab' ib'
-    apply Or.elim (star_star_inv R_functional a b sab b' sab') <;> grind
+    apply Or.elim (star_star_inv R_functional sab b' sab') <;> grind
 
-@[grind ]theorem infseq_star_inv (R_functional : ∀ a b c, R a b -> R a c -> b = c) : ∀ a b, star R a b → infseq R a → infseq R b := by
+@[grind] theorem infseq_star_inv (R_functional : ∀ a b c, R a b -> R a c -> b = c) : ∀ a b, star R a b → infseq R a → infseq R b := by
   intro a b sab ia
-  induction sab
-  case star_refl => grind
-  case star_step x y z rxy syz ih =>
-    unfold infseq at ia
-    grind
+  induction sab with grind [infseq]
 
 theorem infseq_finseq_excl (R_functional : ∀ a b c, R a b -> R a c -> b = c): ∀ a b, star R a b → irred R b → infseq R a → False := by
   intro a b sab irb ia
   have h : infseq R b := by grind
-  unfold infseq at h
-  grind
+  grind [infseq]
 
 theorem infseq_all_seq_inf (R_functional : ∀ a b c, R a b -> R a c -> b = c): ∀ a, infseq R a → all_seq_inf R a := by
   intro a ia
   unfold all_seq_inf
   intro b sab
   have h : infseq R b := by grind
-  unfold infseq at h
-  grind
+  grind [infseq]
